\documentclass{article}

\usepackage{incertia}

% setup the header
\pagestyle{fancy}
\lhead{Will Song}
\chead{Math 427}
\rhead{HW5}

\begin{document}

\begin{enumerate}

\item If $n \in H \leq \ZZ$, then one of $n, -n \geq 0$ so we can take
the smallest positive element of $H$, which we shall name $d$. Clearly
$d\ZZ \leq H$. Now suppose there is some $c$ not in $d\ZZ$ but in $H$.
Then $c = qd + r$ with $0 < r < d$, so $H \ni r = c - qd > 0$
contradicts the minimality of $d$.

\item $H = \lbrace \id, (12) \rbrace$. By Lagrange's Theorem, we have
$\frac{6}{2} = 3$ cosets. The right cosets are
\[ H \backslash G = \lbrace \lbrace \id, (12) \rbrace, \lbrace (23),
(123) \rbrace, \lbrace (31), (321) \rbrace \rbrace. \]
The left cosets are
\[ G / H = \lbrace \lbrace \id, (12) \rbrace, \lbrace (23), (321)
\rbrace, \lbrace (31), (123) \rbrace \rbrace. \]
Left cosets are not right cosets so $H$ is not normal in $S_3$.

\item We cannot find $f^{-1}(1)$ because $f(n) > 1$.

We can define a left inverse $g : \NN \to \NN, 1 \mapsto 1, 1 < n
\mapsto n - 1$ such that $g \circ f = \id_\NN$, but we cannot have a
right inverse because there is no $k \in \NN$ such that $f(k) = 1$.

\item
\begin{enumerate}[(a)]
\item $\varphi_g \circ \varphi_{g^{-1}} = \id = \varphi_{g^{-1}} \circ
\varphi_g$. This is true by compatibility of group action (we get the
trivial action under composition.

\item $\Phi(gh) = \varphi_{gh} = \varphi_g \circ \varphi_h = \Phi(g)
\circ \Phi(h)$.
\end{enumerate}

\item We have both compatability and identity from the group axioms.
i.e. $e \cdot g = eg = g$ and $(gh) \cdot x = g \cdot (h \cdot x)$ from
associativity.

\item For compatability, $(gh) \cdot x = (gh)x(gh)^{-1} =
g(hxh^{-1})g^{-1} = g \cdot (h \cdot x)$. Identity is trivial.

\item Because $\lvert G / H \rvert = 2$, $H$ is normal and $G / H =
\lbrace H, G \setminus H = K \rbrace$. If we want $\ker \varphi = H$,
then we just define $\varphi : H \ni h \mapsto 1, K \ni k \mapsto -1$.
Because $H$ is the identity in the group $G / H$, $K \cdot K = H$ must
be true and $\varphi((k_1h_1)(k_2h_2)) = \varphi(h_3 h_4) = 1$ by
definition. It is easy to check that $\varphi(hk) = -1$ so $\varphi$ is
a homomorphism and we are done.

\item $hkh^{-1}k^{-1} = k_2k^{-1} \in K$ and $hkh^{-1}k^{-1} = hh_2 \in
H$ by normality on $H$ and $K$ so we get $hkh^{-1}k^{-1} \in H \cap K$,
or $hkh^{-1}k^{-1} = e \implies hk = kh$.

\end{enumerate}

\end{document}
